code/bpt_proofs.v
@@ -1,0 +1,35 @@
+Require Export bplustree.
+
+Example kvl_sorted_empty : @kvl_sorted nat [].
+Proof. apply kvl_sorted_0. Qed.
+Example kvl_sorted_single : kvl_sorted [(1, 1)].
+Proof. apply kvl_sorted_1. Qed.
+Example kvl_sorted_two : kvl_sorted [(1, 1), (2, 2)].
+Proof. apply kvl_sorted_cons. apply kvl_sorted_1. reflexivity. Qed.
+Example kvl_sorted_two_WRONG : kvl_sorted [(2, 2), (1, 1)] -> False.
+Proof. unfold not. intro. inversion H. inversion H6. Qed.
+
+Theorem insert_preserves_sort : forall (X: Type) (l: list (nat * X)) (k: nat) (v: X),
+  kvl_sorted l -> kvl_sorted (insert_into_list k v l).
+Proof.
+  intros. induction l. 
+  Case "l = []". simpl. apply kvl_sorted_1.
+  Case "l = a::l". simpl. destruct a. remember (ble_nat k n) as klen. destruct klen.
+    SCase "k <= n". remember (beq_nat k n) as keqn. destruct keqn.
+      SSCase "k = n". symmetry in Heqkeqn. apply beq_nat_true_iff in Heqkeqn. rewrite Heqkeqn. admit.
+      
+      SSCase "k != n". apply kvl_sorted_cons. apply H. 
+                       symmetry in Heqklen. apply ble_nat_true in Heqklen. 
+                       symmetry in Heqkeqn. apply beq_nat_false_iff in Heqkeqn.
+                       apply blt_nat_true. omega.
+    SCase "k > n". 
+    admit.
+Admitted.
+
+Theorem insert_works : forall (X: Type) (l: list (nat * X)) (k: nat) (v: X),
+  search_leaf k (insert_into_list k v l) = Some v. 
+Proof.
+  intros. induction l.
+  Case "l = []". simpl. rewrite <- beq_nat_refl. reflexivity.
+  Case "l = a::l".  simpl. destruct a. remember (ble_nat k n) as keq. destruct keq.
+    rewrite <- Heqkeq.
