code/helper_proofs.v
@@ -1,0 +1,42 @@
+Require Export SfLib.
+
+(* 
+ * Proofs about less-than
+ *)
+Definition blt_nat (n m : nat) : bool :=
+  ble_nat (S n) m.
+  
+Theorem ble_nat_refl : forall n,
+    ble_nat n n = true.
+Proof.
+  induction n. reflexivity.
+  simpl. apply IHn.
+Qed.
+  
+Theorem Sn_lt_Sm__n_lt_m : forall n m,
+  S n < S m -> n < m.
+Proof.
+  induction n. intros m H. omega.
+  intros m H. destruct m. inversion H. inversion H1. omega.
+Qed.
+
+Theorem n_lt_m__Sn_lt_Sm : forall n m,
+  n < m -> S n < S m.
+Proof.
+  intros. induction H; omega.
+Qed.
+ 
+Theorem blt_nat_true : forall n m,
+  blt_nat n m = true <-> n < m.
+Proof. 
+  split; generalize dependent m.
+  Case "->".
+    induction n.  intros m H.
+    destruct m. inversion H. omega.
+    intros m H. destruct m. inversion H. apply n_lt_m__Sn_lt_Sm. apply IHn. rewrite <- H.
+    reflexivity.
+  Case "<-".
+    induction n. intros m H. destruct m. inversion H. unfold blt_nat. simpl. reflexivity.
+    intros m H. destruct m. inversion H. apply Sn_lt_Sm__n_lt_m in H. admit.
+    
+Admitted.
